theories/Eq/UpToTaus.v
@@ -27,8 +27,7 @@ From Coq Require Import
      Relations.Relations.
 
 From ITree Require Import
-     Core
-     UpToTausExplicit.
+     Core.
 
 From ITree Require Export
      Eq.Eq.
@@ -48,7 +47,7 @@ Inductive euttF
       (RBASE: RR r1 r2):
     euttF eutt eutt_taus (RetF r1) (RetF r2)
 | euttF_vis u (e : E u) k1 k2
-      (EUTTK: forall x, eutt (k1 x) (k2 x)):
+      (EUTTK: forall x, eutt (k1 x) (k2 x) \/ eutt_taus (observe (k1 x)) (observe (k2 x))):
     euttF eutt eutt_taus (VisF e k1) (VisF e k2)
 | euttF_tau_tau t1 t2
       (EQTAUS: eutt_taus (observe t1) (observe t2)):
@@ -72,6 +71,7 @@ Lemma euttF_mon r r' s s' x y
   euttF r' s' x y.
 Proof.
   induction EUTT; eauto.
+  econstructor; intros. edestruct EUTTK; eauto.
 Qed.
 
 Lemma monotone_euttF eutt : monotone2 (euttF eutt).
@@ -118,7 +118,7 @@ Global Instance Reflexive_eutt_gen `{Reflexive _ RR}
   Reflexive (paco2 (eutt_ RR) r).
 Proof.
   pcofix CIH. intros. pfold. revert x. pcofix CIH'. intros.
-  genobs x ox. destruct ox; eauto.
+  genobs_clear x ox. destruct ox; eauto 7.
 Qed.
 
 Global Instance Reflexive_euttF_gen `{Reflexive _ RR}
@@ -138,13 +138,50 @@ Proof.
   punfold H1. punfold H1. pfold.
   genobs_clear x ox. genobs_clear y oy.
   induction H1; pclearbot; eauto.
-  - econstructor. intros. destruct (EUTTK x); eauto.
+  - econstructor. intros.
+    edestruct EUTTK as [TMP | TMP]; destruct TMP; eauto 7; contradiction.
   - punfold EQTAUS. eauto 8.
 Qed.
 
 End EUTT_homo.
 
-Lemma Symmetric_eutt_ {E R1 R2}
+Section EUTT_hetero.
+
+Context {E : Type -> Type}.
+
+Lemma Symmetric_euttF_hetero {R1 R2}
+      (RR1 : R1 -> R2 -> Prop) (RR2 : R2 -> R1 -> Prop)
+      (r1 : _ -> _ -> Prop) (r2 : _ -> _ -> Prop) (r'1 : _ -> _ -> Prop) (r'2 : _ -> _ -> Prop)
+      (SYM_RR : forall r1 r2, RR1 r1 r2 -> RR2 r2 r1)
+      (SYM_r : forall i j, r1 i j -> r2 j i)
+      (SYM_r' : forall i j, r'1 i j -> r'2 j i) :
+  forall (ot1 : itree' E R1) (ot2 : itree' E R2),
+    euttF RR1 r1 r'1 ot1 ot2 -> euttF RR2 r2 r'2 ot2 ot1.
+Proof.
+  intros. induction H; eauto 7.
+  econstructor; intros. edestruct EUTTK; eauto 7.
+Qed.
+
+Lemma Symmetric_eutt__hetero {R1 R2}
+      (RR1 : R1 -> R2 -> Prop) (RR2 : R2 -> R1 -> Prop)
+      (r1 : _ -> _ -> Prop) (r2 : _ -> _ -> Prop) (r'1 : _ -> _ -> Prop) (r'2 : _ -> _ -> Prop)
+      (SYM_RR : forall r1 r2, RR1 r1 r2 -> RR2 r2 r1)
+      (SYM_r : forall i j, r1 i j -> r2 j i)
+      (SYM_r' : forall i j, r'1 i j -> r'2 j i) :  
+  forall (ot1 : itree' E R1) (ot2 : itree' E R2),
+    paco2 (euttF RR1 r1) r'1 ot1 ot2 ->
+    paco2 (euttF RR2 r2) r'2 ot2 ot1.
+Proof.
+  pcofix CIH. intros.
+  pfold. punfold H0. 
+  induction H0; pclearbot; eauto 7.
+  - econstructor. intros.
+    edestruct EUTTK; eauto.
+    destruct H; eauto.
+  - destruct EQTAUS; eauto.
+Qed.
+
+Lemma Symmetric_eutt_hetero {R1 R2}
       (RR1 : R1 -> R2 -> Prop) (RR2 : R2 -> R1 -> Prop)
       (r1 : _ -> _ -> Prop) (r2 : _ -> _ -> Prop)
       (SYM_RR : forall r1 r2, RR1 r1 r2 -> RR2 r2 r1)
@@ -157,160 +194,209 @@ Proof.
   pfold. do 2 punfold H0.
   genobs_clear t1 ot1. genobs_clear t2 ot2.
   induction H0; pclearbot; eauto 7.
-  econstructor; intros. edestruct EUTTK; eauto.
+  econstructor; intros.
+  edestruct EUTTK as [TMP | TMP]; destruct TMP; eauto 7; contradiction.
 Qed.
 
-Section EUTT_eq_EUTTE.
+Lemma euttF_elim_tau_left {R1 R2} (RR: R1 -> R2 -> Prop) r (t1: itree E R1) (ot2: itree' E R2)
+    (REL : euttF RR r (upaco2 (euttF RR r) bot2) (TauF t1) ot2) :
+  euttF RR r (upaco2 (euttF RR r) bot2) (observe t1) ot2.
+Proof.
+  remember (TauF t1) as ott1.
+  move REL before r. revert_until REL.
+  induction REL; intros; subst; try dependent destruction Heqott1; eauto.
+  pclearbot. punfold EQTAUS.
+Qed.
+
+Lemma euttF_elim_tau_right {R1 R2} (RR: R1 -> R2 -> Prop) r (ot1: itree' E R1) (t2: itree E R2)
+    (REL : euttF RR r (upaco2 (euttF RR r) bot2) ot1 (TauF t2)) :
+  euttF RR r (upaco2 (euttF RR r) bot2) ot1 (observe t2).
+Proof.
+  eapply (Symmetric_euttF_hetero _ (flip RR) _ (flip r)) in REL; eauto.
+  - eapply euttF_elim_tau_left in REL.
+    eapply Symmetric_euttF_hetero in REL; eauto.
+    intros. pclearbot. left.
+    eapply Symmetric_eutt__hetero; eauto; unfold flip; eauto.
+  - intros. pclearbot. left.
+    eapply Symmetric_eutt__hetero; eauto; unfold flip; eauto.
+Qed.
+
+Definition isb_tau {E R} (ot: itree' E R) : bool :=
+  match ot with | TauF _ => true | _ => false end.
+
+Lemma eutt_Ret {R1 R2} (RR: R1 -> R2 -> Prop) x y :
+  RR x y -> @eutt E R1 R2 RR (Ret x) (Ret y).
+Proof.
+  intros; pfold. pfold. econstructor. eauto.
+Qed.
+
+Lemma eutt_Vis {R1 R2 U} RR (e: E U) k k' :
+  (forall x: U, @eutt E R1 R2 RR (k x) (k' x)) ->
+  eutt RR (Vis e k) (Vis e k').
+Proof.
+  intros. pfold. pfold. econstructor.
+  intros. left. left. apply H.
+Qed.
+
+End EUTT_hetero.
+
+Section EUTT_upto.
 
 Context {E : Type -> Type} {R1 R2 : Type} (RR : R1 -> R2 -> Prop).
 
-Lemma euttE__impl_eutt_ r t1 t2 :
-  @euttE_ E R1 R2 RR r t1 t2 -> eutt_ RR r t1 t2.
-Proof.
-  revert t1 t2. pcofix CIH'. intros. destruct H0.
-  genobs t1 ot1. genobs t2 ot2. clear Heqot1 t1 Heqot2 t2.
-  assert (EM: notauF ot1 \/ notauF ot2 \/ ~(notauF ot1 \/ notauF ot2))
-    by (destruct ot1, ot2; simpl; tauto).
-  destruct EM as [EM|[EM|EM]].
-  - destruct FIN as [FIN _].
-    hexploit FIN; eauto 7. clear FIN; intro FIN.
-    destruct FIN as [ot' [UNTAUS NOTAU]].
-    hexploit EQV; eauto. intros EQNT.
-    induction UNTAUS; subst.
-    { pfold. inv EQNT; eauto. }
-    hexploit IHUNTAUS; eauto.
-    { intros. destruct UNTAUS1.
-      dependent destruction H; [|subst; contradiction].
-      hexploit @unalltaus_injective; [|econstructor|]; eauto. intros; subst; eauto.
-    }
-    intros EUTT. punfold EUTT.
-  - destruct FIN as [_ FIN].
-    hexploit FIN; eauto 7. clear FIN; intro FIN.
-    destruct FIN as [ot' [UNTAUS NOTAU]].
-    hexploit EQV; eauto. intros EQNT.
-    induction UNTAUS; subst.
-    { pfold. inv EQNT; eauto. }
-    hexploit IHUNTAUS; eauto.
-    { intros. destruct UNTAUS2.
-      dependent destruction H; [|subst; contradiction].
-      hexploit @unalltaus_injective; [|econstructor|]; eauto. intros; subst; eauto.
-    }
-    intros EUTT. punfold EUTT.
-  - destruct ot1, ot2; simpl in *; try tauto.
-    pfold. econstructor. right. apply CIH'.
-    econstructor.
-    + rewrite !finite_taus_tau in FIN. eauto.
-    + eauto using unalltaus_tau'.
-Qed.
-
-Lemma eutt__impl_euttE_ r t1 t2 :
-  @eutt_ E R1 R2 RR r t1 t2 -> euttE_ RR r t1 t2.
-Proof.
-  intros. punfold H. econstructor; intros.
-  - split; intros.
-    + genobs t1 ot1. genobs t2 ot2. clear Heqot1 t1 Heqot2 t2.
-      destruct H0 as [ot' [UNTAUS NOTAU]].
-      move UNTAUS before r. revert_until UNTAUS.
-      induction UNTAUS; intros.
-      * induction H; eauto; try contradiction.
-        rewrite finite_taus_tau. eauto.
-      * induction H; eauto 7; try inv OBS; pclearbot
-        ; rewrite ?finite_taus_tau; eauto; eapply IHUNTAUS; eauto.
-        punfold EQTAUS.
-   + genobs t1 ot1. genobs t2 ot2. clear Heqot1 t1 Heqot2 t2.
-     destruct H0 as [ot' [UNTAUS NOTAU]].
-     move UNTAUS before r. revert_until UNTAUS.
-     induction UNTAUS; intros.
-     * induction H; eauto; try contradiction.
-       rewrite finite_taus_tau. eauto.
-     * induction H; eauto 7; try inv OBS; pclearbot
-       ; rewrite ?finite_taus_tau; eauto; eapply IHUNTAUS; eauto.
-       punfold EQTAUS.
-  - genobs t1 ot1. genobs t2 ot2. clear Heqot1 t1 Heqot2 t2.
-    destruct UNTAUS1 as [UNTAUS1 NT1]. destruct UNTAUS2 as [UNTAUS2 NT2].
-    move UNTAUS2 before r. move UNTAUS1 before r. revert_until UNTAUS1.
-    induction UNTAUS1.
-    + induction 1; intros.
-      * inv H; try contradiction; eauto.
-      * subst. inv H; try contradiction. eauto.
-    + induction 1; intros; subst.
-      * inv H; try contradiction; eauto.
-      * inv H; try contradiction; eauto.
-        pclearbot. eapply IHUNTAUS1; eauto.
-        punfold EQTAUS.
-Qed.
-
-Lemma eutt__is_euttE_ r t1 t2 :
-  @eutt_ E R1 R2 RR r t1 t2 <-> euttE_ RR r t1 t2.
-Proof. split; eauto using euttE__impl_eutt_, eutt__impl_euttE_. Qed.
-
-Lemma euttE_impl_eutt r t1 t2 :
-  paco2 (@euttE_ E R1 R2 RR) r t1 t2 -> paco2 (eutt_ RR) r t1 t2.
-Proof.
-  split; intros; eapply paco2_mon_gen; eauto; intros; apply euttE__impl_eutt_; eauto.
-Qed.
-
-Lemma eutt_impl_euttE r t1 t2 :
-  paco2 (@eutt_ E R1 R2 RR) r t1 t2 -> paco2 (euttE_ RR) r t1 t2.
-Proof.
-  split; intros; eapply paco2_mon_gen; eauto; intros; apply eutt__impl_euttE_; eauto.
-Qed.
-
-Lemma eutt_is_euttE r t1 t2 :
-  paco2 (@eutt_ E R1 R2 RR) r t1 t2 <-> paco2 (euttE_ RR) r t1 t2.
-Proof. split; eauto using euttE_impl_eutt, eutt_impl_euttE. Qed.
-
-End EUTT_eq_EUTTE.
-
-Section EUTT_trans.
-
-Context {E : Type -> Type} {R1 R2 : Type} (RR : R1 -> R2 -> Prop).
-
-Ltac convert_eutt_to_euttE :=
-  try (apply euttE__impl_eutt_ || apply euttE_impl_eutt);
-  repeat match goal with [H: eutt_ _ _ _ _ |- _] => apply eutt__impl_euttE_ in H end;
-  repeat match goal with [H: eutt _ _ _ |- _] => apply eutt_impl_euttE in H end.
-
-Inductive eutt_trans_clo (r: itree E R1 -> itree E R2 -> Prop) :
+Inductive eutt_trans_left_clo (r: itree E R1 -> itree E R2 -> Prop) :
   itree E R1 -> itree E R2 -> Prop :=
-| eutt_pre_clo_intro t1 t2 t3 t4
-      (EQVl: t1 ≈ t2)
-      (EQVr: t4 ≈ t3)
+| eutt_trans_left_clo_intro t1 t2 t3
+      (EQV: t1 ≈ t2)
       (REL: r t2 t3)
-  : eutt_trans_clo r t1 t4
+  : eutt_trans_left_clo r t1 t3
 .
-Hint Constructors eutt_trans_clo.
+Hint Constructors eutt_trans_left_clo.
 
-Lemma eutt_clo_trans :
-  weak_respectful2 (@eutt_ E R1 R2 RR) eutt_trans_clo.
+Lemma eutt_clo_trans_left :
+  weak_respectful2 (@eutt_ E R1 R2 RR) eutt_trans_left_clo.
 Proof.
   econstructor; [pmonauto|].
   intros. destruct PR.
-  convert_eutt_to_euttE.
-  destruct (euttE_clo_trans E _ _ RR). clear WEAK_MON.
-  hexploit WEAK_RESPECTFUL.
-  { apply LE. }
-  { intros. apply GF in PR. convert_eutt_to_euttE. auto. }
-  { econstructor; [apply EQVl|apply EQVr|apply REL]. }
-  intros EUTT.
-  eapply monotone_euttE_; eauto; intros.
-  eapply rclo2_mon_gen; eauto; intros.
-  - convert_eutt_to_euttE. auto.
-  - destruct PR0. econstructor; convert_eutt_to_euttE; eauto.
+  eapply GF in REL. clear l LE GF.
+  revert_until r. pcofix CIH. intros.
+  pfold. punfold REL. do 2 punfold EQV.
+  genobs_clear t1 ot1. genobs_clear t2 ot2. genobs_clear t3 ot3.
+  move EQV before CIH. revert_until EQV.
+  induction EQV; intros; subst; pclearbot; eauto 7 using euttF_mon, upaco2_mon_bot, rclo2.
+  - remember (VisF e k2) as o.
+    move REL before CIH. revert_until REL.
+    induction REL; intros; subst; try dependent destruction Heqo; pclearbot; eauto 7.
+    econstructor. intros.
+    edestruct EUTTK, EUTTK0; pclearbot; eauto 7 using rclo2.
+  - destruct (isb_tau ot3) eqn: ISTAU.
+    + destruct ot3; inv ISTAU.
+      econstructor. right. eapply CIH. eauto.
+      pfold.
+      eapply euttF_elim_tau_left in REL.
+      eapply euttF_elim_tau_right in REL. eauto.
+    + dependent destruction REL; simpobs; inv ISTAU.
+      econstructor. genobs_clear t2 ot.
+      move REL before CIH. revert_until REL.
+      induction REL; intros; inv H0.
+      * punfold EQTAUS.
+        genobs_clear t1 ot1. remember (RetF r1) as o.
+        move EQTAUS before CIH. revert_until EQTAUS.
+        induction EQTAUS; intros; subst; try dependent destruction Heqo; pclearbot; eauto 7.
+      * punfold EQTAUS.
+        genobs_clear t1 ot1. remember (VisF e k1) as o.
+        move EQTAUS before CIH. revert_until EQTAUS.
+        induction EQTAUS; intros; subst; try dependent destruction Heqo; pclearbot; eauto 7.
+        econstructor. intros.
+        edestruct EUTTK, EUTTK0; pclearbot; eauto 7 using rclo2.
+      * eapply IHREL; eauto.
+        punfold EQTAUS. pfold.
+        eapply euttF_elim_tau_right in EQTAUS. eauto.
+  - remember (TauF t2) as o.
+    move REL before CIH. revert_until REL.
+    induction REL; intros; subst; try dependent destruction Heqo; pclearbot; eauto 7.
+    punfold EQTAUS.
+Qed.
+
+Inductive eutt_trans_right_clo (r: itree E R1 -> itree E R2 -> Prop) :
+  itree E R1 -> itree E R2 -> Prop :=
+| eutt_trans_right_clo_intro t1 t2 t3
+      (EQV: t3 ≈ t2)
+      (REL: r t1 t2)
+  : eutt_trans_right_clo r t1 t3
+.
+Hint Constructors eutt_trans_right_clo.
+
+Lemma eutt_clo_trans_right :
+  weak_respectful2 (@eutt_ E R1 R2 RR) eutt_trans_right_clo.
+Proof.
+  econstructor; [pmonauto|].
+  intros. destruct PR.
+  eapply GF in REL. clear l LE GF.
+  revert_until r. pcofix CIH. intros.
+  pfold. punfold REL. do 2 punfold EQV.
+  genobs_clear t1 ot1. genobs_clear t2 ot2. genobs_clear t3 ot3.
+  move EQV before CIH. revert_until EQV.
+  induction EQV; intros; subst; pclearbot; eauto 7 using euttF_mon, upaco2_mon_bot, rclo2.
+  - remember (VisF e k2) as o.
+    move REL before CIH. revert_until REL.
+    induction REL; intros; subst; try dependent destruction Heqo; pclearbot; eauto 7.
+    econstructor. intros.
+    edestruct EUTTK, EUTTK0; pclearbot; eauto 7 using rclo2.
+  - destruct (isb_tau ot1) eqn: ISTAU.
+    + destruct ot1; inv ISTAU.
+      econstructor. right. eapply CIH. eauto.
+      pfold.
+      eapply euttF_elim_tau_left in REL.
+      eapply euttF_elim_tau_right in REL. eauto.
+    + dependent destruction REL; simpobs; inv ISTAU.
+      econstructor. genobs_clear t2 ot.
+      move REL before CIH. revert_until REL.
+      induction REL; intros; inv H0.
+      * punfold EQTAUS.
+        remember (RetF r2) as o.
+        move EQTAUS before CIH. revert_until EQTAUS.
+        induction EQTAUS; intros; subst; try dependent destruction Heqo; pclearbot; eauto 7.
+      * punfold EQTAUS.
+        remember (VisF e k2) as o.
+        move EQTAUS before CIH. revert_until EQTAUS.
+        induction EQTAUS; intros; subst; try dependent destruction Heqo; pclearbot; eauto 7.
+        econstructor. intros.
+        edestruct EUTTK, EUTTK0; pclearbot; eauto 7 using rclo2.
+      * eapply IHREL; eauto.
+        punfold EQTAUS. pfold.
+        eapply euttF_elim_tau_right in EQTAUS. eauto.
+  - remember (TauF t2) as o.
+    move REL before CIH. revert_until REL.
+    induction REL; intros; subst; try dependent destruction Heqo; pclearbot; eauto 7.
+    punfold EQTAUS.
+Qed.
+
+Inductive eutt_bind_clo {E R1 R2} (r: itree E R1 -> itree E R2 -> Prop) : itree E R1 -> itree E R2 -> Prop :=
+| eutt_bind_clo_intro U1 U2 RU t1 t2 k1 k2
+      (EQV: @eutt E U1 U2 RU t1 t2)
+      (REL: forall v1 v2 (RELv: RU v1 v2), r (k1 v1) (k2 v2))
+  : eutt_bind_clo r (ITree.bind t1 k1) (ITree.bind t2 k2)
+.
+Hint Constructors eutt_bind_clo.
+
+Lemma eutt_clo_bind : weak_respectful2 (@eutt_ E R1 R2 RR) eutt_bind_clo.
+Proof.
+  econstructor; [pmonauto|].
+  intros. destruct PR.
+  assert (RELk: forall v1 v2, RU v1 v2 -> eutt_ RR r (k1 v1) (k2 v2)) by eauto.
+  clear l LE GF REL.
+  revert_until r. pcofix CIH. intros.
+  pfold. do 2 punfold EQV.
+  rewrite !unfold_bind.
+  genobs_clear t1 ot1. genobs_clear t2 ot2.
+  move EQV before CIH. revert_until EQV.
+  induction EQV; intros; subst; pclearbot.
+  - specialize (RELk _ _ RBASE). punfold RELk.
+    eauto 7 using euttF_mon, upaco2_mon_bot, rclo2.
+  - econstructor. intros.
+    edestruct EUTTK; pclearbot; eauto 7 using rclo2.
+  - simpl. eauto 7.
+  - econstructor. rewrite unfold_bind. eauto.
+  - econstructor. rewrite unfold_bind. eauto.
 Qed.
 
 Global Instance eutt_cong_eutt r :
   Proper (eutt eq ==> eutt eq ==> flip impl)
          (paco2 (@eutt_ E R1 R2 RR ∘ gres2 (eutt_ RR)) r).
 Proof.
-  repeat intro. pupto2 eutt_clo_trans. eauto.
+  repeat intro.
+  pupto2 eutt_clo_trans_left. econstructor; eauto.
+  pupto2 eutt_clo_trans_right. econstructor; eauto.
 Qed.
 
 Global Instance eutt_cong_gres_eutt_ r :
   Proper (eutt eq ==> eutt eq ==> flip impl)
          (gres2 (@eutt_ E R1 R2 RR) r).
 Proof.
-  repeat intro. pupto2 eutt_clo_trans. eauto.
+  repeat intro.
+  pupto2 eutt_clo_trans_left. econstructor; eauto.
+  pupto2 eutt_clo_trans_right. econstructor; eauto.
 Qed.
 
 Global Instance eutt_eq_under_rr_impl :
@@ -319,18 +405,34 @@ Proof.
   repeat red. intros. pupto2_init. rewrite H, H0. pupto2_final. eauto.
 Qed.
 
-End EUTT_trans.
+End EUTT_upto.
 
-Arguments eutt_clo_trans : clear implicits.
-Hint Constructors eutt_trans_clo.
+Arguments eutt_clo_trans_left : clear implicits.
+Hint Constructors eutt_trans_left_clo.
 
-Section EUTT_nested_trans.
+Arguments eutt_clo_trans_right : clear implicits.
+Hint Constructors eutt_trans_right_clo.
+
+Arguments eutt_clo_bind : clear implicits.
+Hint Constructors eutt_bind_clo.
+
+Global Instance eutt_bind {E U R} :
+  Proper (eutt eq ==>
+          pointwise_relation _ (eutt eq) ==>
+          eutt eq) (@ITree.bind E U R).
+Proof.
+  repeat intro.
+  pupto2_init. pupto2 eutt_clo_bind. econstructor; eauto.
+  intros. subst. pupto2_final. apply H0.
+Qed.
+
+Section EUTT_nested.
 
 Context {E : Type -> Type} {R1 R2 : Type} (RR : R1 -> R2 -> Prop).
 
 Inductive eutt_nested_trans_clo (r: itree' E R1 -> itree' E R2 -> Prop) :
   itree' E R1 -> itree' E R2 -> Prop :=
-| eutt_nested_pre_clo_intro ot1 ot2 ot3 ot4
+| eutt_nested_trans_clo_intro ot1 ot2 ot3 ot4
       (EQVl: go ot1 ≅ go ot2)
       (EQVr: go ot4 ≅ go ot3)
       (REL: r ot2 ot3)
@@ -350,7 +452,14 @@ Proof.
   induction REL; intros; subst;
     try (dependent destruction EQVl; dependent destruction EQVr; [ idtac ]; pclearbot).
   - eauto.
-  - econstructor. intros. rewrite REL, REL0. eauto.
+  - econstructor. intros.
+    edestruct EUTTK.
+    + left. rewrite REL, REL0. eauto.
+    + right. eapply rclo2_step.
+      econstructor.
+      * instantiate (1:= observe(k1 x)). rewrite <- !itree_eta. eauto.
+      * instantiate (1:= observe(k2 x)). rewrite <- !itree_eta. eauto.
+      * eauto using rclo2.
   - econstructor. eapply rclo2_step. econstructor.
     + rewrite REL. reflexivity.
     + rewrite REL0. reflexivity.
@@ -368,10 +477,43 @@ Proof.
   pupto2 eutt_nested_clo_trans. econstructor; eauto.
 Qed.
 
-End EUTT_nested_trans.
+Inductive eutt_nested_bind_clo (r: itree' E R1 -> itree' E R2 -> Prop) : itree' E R1 -> itree' E R2 -> Prop :=
+| eutt_nested_bind_clo_intro U1 U2 RU t1 t2 k1 k2
+      (EQV: @eutt E U1 U2 RU t1 t2)
+      (REL: forall v1 v2 (RELv: RU v1 v2), r (observe (k1 v1)) (observe (k2 v2)))
+  : eutt_nested_bind_clo r (observe (ITree.bind t1 k1)) (observe (ITree.bind t2 k2))
+.
+Hint Constructors eutt_nested_bind_clo.
+
+Lemma eutt_nested_clo_bind r :
+  weak_respectful2 (euttF RR (gres2 (eutt_ RR) (upaco2 (eutt_ RR ∘ gres2 (eutt_ RR)) r)))
+                    eutt_nested_bind_clo.
+Proof.
+  econstructor; [pmonauto|].
+  intros. destruct PR.
+  assert (RELk: forall v1 v2, RU v1 v2 -> euttF RR (gres2 (eutt_ RR) (upaco2 (eutt_ RR ∘ gres2 (eutt_ RR)) r)) r0 (observe (k1 v1)) (observe (k2 v2))) by eauto.
+  clear l LE GF REL.
+  do 2 punfold EQV.
+  rewrite !unfold_bind.
+  genobs_clear t1 ot1. genobs_clear t2 ot2.
+  move EQV before RU. revert_until EQV.
+  induction EQV; intros; subst; pclearbot.
+  - specialize (RELk _ _ RBASE). 
+    eauto 7 using euttF_mon, upaco2_mon_bot, rclo2.
+  - econstructor. intros.
+    edestruct EUTTK; pclearbot; eauto 8 using rclo2.
+  - simpl. eauto 9 using rclo2.
+  - econstructor. rewrite unfold_bind. eauto.
+  - econstructor. rewrite unfold_bind. eauto.
+Qed.
+
+End EUTT_nested.
 
 Arguments eutt_nested_clo_trans : clear implicits.
 Hint Constructors eutt_nested_trans_clo.
+
+Arguments eutt_nested_clo_bind : clear implicits.
+Hint Constructors eutt_nested_bind_clo.
 
 Section EUTT_eq.
 
@@ -446,26 +588,6 @@ Proof.
   intros. pfold. pfold. econstructor. eauto.
 Qed.
 
-Global Instance eutt_bind {E S R} :
-  Proper (eutt eq ==>
-          pointwise_relation _ (eutt eq) ==>
-          eutt eq) (@ITree.bind E R S).
-Proof.
-  repeat intro. do 2 punfold H.
-  revert_until S. pcofix CIH. intros.
-  pfold. revert_until CIH. pcofix CIH'. intros. pfold.
-  rewrite !unfold_bind. genobs_clear x ox. genobs_clear y oy.
-  move H0 before CIH'. revert_until H0.
-  induction H0; intros; subst; pclearbot.
-  - simpl. specialize (H1 r2). do 2 punfold H1.
-    eauto 7 using euttF_mon, upaco2_mon_bot.
-  - econstructor. intros.
-    specialize (EUTTK x). do 2 punfold EUTTK.
-  - econstructor. intros. punfold EQTAUS.
-  - econstructor. rewrite unfold_bind. eauto.
-  - econstructor. rewrite unfold_bind. eauto.
-Qed.
-
 Global Instance eutt_map {E R S} :
   Proper (pointwise_relation _ eq ==> eutt eq ==> eutt eq) (@ITree.map E R S).
 Proof.
@@ -476,20 +598,11 @@ Qed.
 Global Instance eutt_forever {E R S} :
   Proper (eutt eq ==> eutt eq) (@ITree.forever E R S).
 Proof.
-  cut (forall X (t1 t2: itree E X) (x y: itree E R), t1 ≈ t2 -> x ≈ y -> (t1 ;; @ITree.forever E R S x) ≈ (t2 ;; ITree.forever y)).
-  { repeat intro.
-    rewrite <-(ret_bind tt (fun _ => ITree.forever x)).
-    rewrite <-(ret_bind tt (fun _ => ITree.forever y)).
-    eapply H; eauto; reflexivity.
-  }
-
-  pcofix CIH. intros. 
-  pfold. revert_until CIH. pcofix CIH'. intros.
-  do 2 punfold H0. pfold.
-  rewrite !unfold_bind. genobs_clear t1 ot1. genobs_clear t2 ot2.
-  induction H0; intros; subst; pclearbot; try (econstructor; eauto 7; fail).
-  simpl. rewrite (unfold_forever x), (unfold_forever y). 
-  econstructor. eauto 7.
+  repeat intro. pupto2_init. revert_until S. pcofix CIH. intros.
+  pfold. pupto2_init. revert_until CIH. pcofix CIH'. intros.
+  rewrite (unfold_forever x), (unfold_forever y).
+  pupto2 eutt_nested_clo_bind. econstructor; eauto.
+  intros. subst. pupto2_final. pfold. simpl. eauto.
 Qed.
 
 Global Instance eutt_when {E} (b : bool) :
@@ -509,4 +622,15 @@ Qed.
 Lemma tau_eutt {E R} (t: itree E R) : Tau t ≈ t.
 Proof.
   pfold. pfold. econstructor. reflexivity.
+Qed.
+
+(** Generalized heterogeneous version of [eutt_bind] *)
+Lemma eutt_bind_gen {E R1 R2 S1 S2} {RR: R1 -> R2 -> Prop} {SS: S1 -> S2 -> Prop}:
+  forall t1 t2,
+    eutt RR t1 t2 ->
+    forall s1 s2, (forall r1 r2, RR r1 r2 -> eutt SS (s1 r1) (s2 r2)) ->
+                  @eutt E _ _ SS (ITree.bind t1 s1) (ITree.bind t2 s2).
+Proof.
+  intros. red in H0. pupto2_init. pupto2 eutt_clo_bind. econstructor; eauto.
+  intros. pupto2_final. eauto.
 Qed.
